<p>The following theorem will be very useful to derive basic properties of entropy.</p>
<div class="content-box pad-box-mini border border-trbl border-round">
<h4 style="color: #bc0031;"><strong>Theorem: Jensen's inequality</strong></h4>
Let \(f : \mathcal{D} \to \mathbb{R}\) be a convex function, and let \(n \in \mathbb{N}\). Then for any \(p_1, \ldots, p_n \in \mathbb{R}_{\geq 0}\) such that \(\sum_{i=1}^n p_i = 1\) and for any \(x_1, \ldots, x_n \in \mathcal{D}\) it holds that \[ \sum_{i=1}^n p_if(x_i) \geq f\left(\sum_{i=1}^np_ix_i\right). \] If \(f\) is strictly convex and \(p_1, \ldots, p_n &gt; 0\), then equality holds if and only if \(x_1 = \cdots = x_n\). In particular, if \(X\) is a real random variable whose image \(\mathcal{X}\) is contained in \(\mathcal{D}\), then \[ \mathbb{E}[f(X)] \geq f(\mathbb{E}[X]), \] and if \(f\) is strictly convex, equality holds if and only if there is a \(c \in \mathcal{X}\) such that \(X = c\) with probability 1.
<p><span class="element_toggler" role="button" aria-controls="group3" aria-label="Toggler" aria-expanded="false"><span class="Button">Show proof</span></span></p>
<div id="group3" style="display: none;">
<div class="content-box">The proof is by induction. The case \(n=1\) is trivial, and the case \(n=2\) is identical to the very definition of convexity. Suppose that we have already proved the claim up to \(n-1 \geq 2\). Assume, <a href="https://en.wikipedia.org/wiki/Without_loss_of_generality" target="_blank">without loss of generality</a>, that \(p_n &lt; 1\). Then: \( \begin{align} \sum_{i=1}^n p_i f(x_i) &amp;= p_n f(x_n) + \sum_{i=1}^{n-1} p_i f(x_i) \\ &amp;= p_n f(x_n) + (1-p_n)\sum_{i=1}^{n-1} \frac{p_i}{1-p_n} f(x_i) \\ &amp;\geq p_n f(x_n) + (1-p_n)f\left(\sum_{i=1}^{n-1} \frac{p_i}{1-p_n} x_i\right) \text{(induction hypothesis)} \\ &amp;\geq f\left(p_n x_n + (1-p_n)\sum_{i=1}^{n-1} \frac{p_i}{1-p_n} x_i\right) \text{(definition of convexity)} \\ &amp;= f\left(p_n x_n + \sum_{i=1}^{n-1} p_i x_i\right) \\&amp;= f\left(\sum_{i=1}^np_ix_i\right). \end{align}\)
<p>That proves the claim. As for the strictness claim, if \(x_1, \ldots, x_n\) are not all identical, then either \(x_1, \ldots, x_{n-1}\) are not all identical and the first inequality is strict by induction hypothesis, or \(x_1 = \cdots = x_{n-1} \neq x_n\) so that the second inequality is strict by the definition of convexity.</p>
</div>
</div>
</div>
<p>Â </p>